Fix Name bug
Problem: the way Name is currently written, we can substitute the wrong 'val'.

Solution: used 'Cached' to fix that. Also made Cached private to enforce a bit
of correctness, though we will almost certainly want to follow it up with Jonn's
efforts on the other branch.

Wasm/Wast/Expr.lean
@@ -66,6 +66,30 @@ inductive NumType :=
 | int : BitSize → NumType
 | float : BitSize → NumType
 
+--------------------------------------------------
+--               Type-level parsing             --
+--------------------------------------------------
+
+section cached
+
+/-
+Cached as a way to enforce that only the one correct value
+is used. We use in in structures representing WAST types to
+enforce correctness of inner values.
+-/
+private def Cached {α : Type u} (a : α) := { cached : α // cached = a }
+
+instance : EmptyCollection (Cached a) where emptyCollection := ⟨a, rfl⟩
+instance : Inhabited (Cached a) where default := {}
+instance : Subsingleton (Cached a) where
+  allEq := fun ⟨b, hb⟩ ⟨c, hc⟩ => by subst hb; subst hc; rfl
+instance : DecidableEq (Cached a) := fun _ _ => isTrue (Subsingleton.allEq ..)
+instance [Repr α] : Repr (Cached (a : α)) where
+  reprPrec c n := reprPrec c.val n
+
+end cached
+
+
 def isDigit (x : Char) : Bool :=
   x.isDigit
 
@@ -135,43 +159,22 @@ private def extractNat' -- (x : String)
 private def parseRadixNat'Do' (_radix : Nat) (input : String) : Either String Nat :=
   if input == "23" then
     .right 100
+  else if input == "45" then .right 45
   else
     .left "Menzoberranzan"
 
 private def demoParse (φ : String → Either String Nat) (x : String) : Either String Nat :=
   φ x
 
-structure Nat' (x : String) :=
-  -- radix := hod x
-  radix := 10
-  valE := demoParse (parseRadixNat'Do' radix) x
-  doesParse : Either.isRight $ demoParse (parseRadixNat'Do' radix) x
-  val : Nat := extractNat' (demoParse (parseRadixNat'Do' radix) x) doesParse
-
-def Cached {α : Type u} (a : α) := { cached : α // cached = a }
-
-instance : EmptyCollection (Cached a) where emptyCollection := ⟨a, rfl⟩
-instance : Inhabited (Cached a) where default := {}
-instance : Subsingleton (Cached a) where
-  allEq := fun ⟨b, hb⟩ ⟨c, hc⟩ => by subst hb; subst hc; rfl
-instance : DecidableEq (Cached a) := fun _ _ => isTrue (Subsingleton.allEq ..)
 
 structure Nat'' (x : String) :=
   radix : Cached (hod x) := {}
   valE : Cached (demoParse (parseRadixNat'Do' radix.val) x) := {}
   doesParse : Either.isRight valE.val := by simp
   val : Cached (extractNat' valE.val doesParse) := {}
-  -- radix := hod x
-  -- valE := demoParse (parseRadixNat'Do' radix) x
-  -- doesParse : Either.isRight $ demoParse (parseRadixNat'Do' radix) x
-  -- val : Nat := extractNat' (demoParse (parseRadixNat'Do' radix) x) doesParse
   deriving DecidableEq
 
 def nobug : Nat'' "23" := {}
--- def bug : Nat'' "45" := {}
-#eval nobug.val
-
-#eval nobug = nobug
 
 -- @[simp] theorem eq_of_subsingleton [Subsingleton α] {a b : α} : (a = b) = True := by
 --   simp [Subsingleton.allEq a b]
@@ -179,8 +182,16 @@ def nobug : Nat'' "23" := {}
 -- theorem extIff {a b : Nat'' x} : a = b ↔ x = x :=
 --    ⟨fun h => by subst h; rfl, by cases a; cases b; intro h; cases h; simp⟩
 
-theorem high_five : Either.isRight $ demoParse (parseRadixNat'Do' $ hod "23") "23" := by
-  simp
+def r : Cached (hod "23") := {}
+def five : Cached (demoParse (parseRadixNat'Do' r.val) "23") := {}
+theorem high_five : Either.isRight $ five.val := by simp
+theorem noparse : Either.isRight $ demoParse (parseRadixNat'Do' (hod "23")) "23" := by simp
+-- def bug : Nat'' "45" := { doesParse := noparse }
+
+
+----------------------------
+--          Name          --
+----------------------------
 
 def isIdChar (x : Char) : Bool :=
   x.isAlphanum || "_.+-*/\\^~=<>!?@#$%&|:'`".data.elem x
@@ -188,9 +199,9 @@ def isIdChar (x : Char) : Bool :=
 /- Captures a valid identifier.
 -/
 structure Name (x : String) where
-  val : String := x
-  isNE : x.length ≠ 0
-  onlyLegal : x.data.all isIdChar
+  val : Cached x := {}
+  isNE : x.length ≠ 0 := by trivial
+  onlyLegal : x.data.all isIdChar := by trivial
   deriving Repr
 
 def mkName (xs : String) : Option (Name xs) :=
